Random updates to coq files, update transform with new ca algo, examples

scheme/transform.rkt
@@ -1,194 +1,123 @@
 #lang racket
 
 (require rackunit)
-(require "lc_enum.rkt")
 
-;assumptions
-;  lambdas have one argument
-;  let has one assignment
-;  all terms are locally closed (no bound variables outside of an abstraction)
+(define (get-assignments store E e)
+  (flatten (append (sf-as-l store) (append (E-as E) (e-as e)))))
 
-(define (has-assigning-set-list i exp-list)
-  (match exp-list
-    ['() #f]
-    [`(,exp)
-     (has-assigning-set i exp)]
-    [`(,e ,es ...)
-     (or (has-assigning-set i e) (has-assigning-set-list i es))]))
+(define (sf-as sf)
+  (match sf
+    [`(,x ,v) (cons x (e-as v))]
+    [u '()]))
 
-(define (has-assigning-set i exp)
-  (match exp
-    [`(set! (bvar ,n) ,e) ;assigning set alone
-     #:when (eq? i n)
-     #t]
-    [`(set! (bvar ,n) ,e ...) ;assigning set
-     #:when (eq? i n)
-     #t]
-    [`(set! (bvar ,n) ,e) (has-assigning-set i e)] ;non-assigning set
-    [`(lam . ,body) (has-assigning-set (+ i 1) body)] ;if let or lambda, increase abs index
-    [`(let ,v ,body) (has-assigning-set (+ i 1) body)]
-    [`(let ,v ,e ...)
-     (has-assigning-set-list (+ i 1) e)]
-    [`(,e1 ,e2) (and (has-assigning-set i e1) (has-assigning-set i e2))] ;if app, check both exprs
-    ;[`(bvar ,n) #f] ;just variables
-    ;[`(fvar ,x) #f]
-    [_ #f]))
+(define (sf-as-l sfs)
+  (match sfs
+    ['() '()]
+    [`(,sf) (list (sf-as sf))]
+    [`(,sf ,sfs1 ...) (cons (sf-as sf) (sf-as-l sfs1))]))
 
-(define (handle-assigning-set-list i exps)
-  (match exps
-    [`() `()]
-    [`(,exp) (handle-assigning-set i exp)]
-    [`(,e ,es ...)
-     `(,(handle-assigning-set i e) ,(handle-assigning-set-list i es))]))
+(define (store-as store)
+  (match store
+    ['() '()]
+    [(cons sf sfs) (cons (sf-as sf) (store-as sfs))]))
 
-(define (handle-assigning-set i exp)
-  (match exp
-    [`(set! (bvar ,n) ,e) ;assigning set
-     #:when (eq? i n)
-     `(set-car! (bvar ,n) ,(handle-assigning-set i e))]
-    [`(set! (bvar ,n) ,e)
-     `(set-top-level! (bvar ,n) ,(handle-assigning-set i e))] ;non-assigning set
-    [`(lam . ,body)
-     `(lam . ,(handle-assigning-set (+ i 1) body))] ;if let or lambda, increase abs index
-    [`(let ,v ,body ...)
-     `(let ,v ,(map (lambda (e)
-                      (handle-assigning-set i e)) body))]
-    [`(bvar ,n)
-     #:when (eq? i n)
-     `(car (bvar ,n))]
-    [`(,e1 ,e2)
-     `(,(handle-assigning-set i e1) ,(handle-assigning-set i e2))] ;if app, handle both exprs
-    [x x]))
+(define (e-as-l es)
+  (match es
+    ['() '()]
+    [(cons e es1) (append (e-as e) (e-as-l es1))]))
 
-(define (op? o)
-  (member o '(+ / * -)))
+(define (E-as E)
+  (match E
+    ['[] '()]
+    [`(set! ,x ,E1) (cons x (E-as E1))]
+    [`(begin ,E1 ,e1 ,e2 ...) (append (E-as E1) (append (e-as e1) (e-as-l e2)))]
+    [`(,v1 ... ,E1 ,v2 ...) (append (E-as E1) (append (e-as-l v1) (e-as-l v2)))]))
 
-(define (convert-assignments-list sfs exps)
-  (match exps
-    [`() `()]
-    [`(,exp) (convert-assignments sfs exp)]
-    [`(,e ,es ...)
-     (list (convert-assignments sfs e) (convert-assignments-list sfs es))]))
+(define (e-as e)
+  (match e
+    [`(begin ,e1 ,e2 ...) (append (e-as e1) (e-as-l e2))]
+    [`(,set! ,x ,e1) (cons x (e-as e1))]
+    [`(λ ,x ,e1) (e-as e1)]
+    [`(,e1 ,e2 ...) (append (e-as e1) (e-as-l e2))]
+    [_ '()]))
 
-;convert assignments pass
-;  sfs is the store
-;  exp is the expression to be transformed
-;  i is the current highest level of abstraction (for debruijn)
-(define (convert-assignments sfs exp)
-  (match exp
-    ;lets with assigning set in body
-    [`(let ,v ,body)
-     #:when (has-assigning-set 0 body)
-     `(let ,v
-        (let (cons (bvar 0) '())
-          ,(convert-assignments sfs (handle-assigning-set 0 body))))]
-    [`(let ,v ,body ...)
-     #:when (has-assigning-set-list 0 body)
-     `(let ,v
-        (let (cons (bvar 0) '())
-          ,(convert-assignments-list sfs (handle-assigning-set-list 0 body))))]
-    ;lets without assigning set in body
-    [`(let ,v ,body)
-     `(let ,v ,(convert-assignments sfs body))]
-    [`(let ,v ,body ...)
-     `(let ,v ,(convert-assignments-list sfs body))]
-    ;app
-    [`(,e1 ,e2)
-     `(,(convert-assignments sfs e1) ,(convert-assignments sfs e2))]
-    ;abs
-    [`(lam . ,body)
-     `(lam . ,(convert-assignments sfs body))]
-    ;top level set
-    [`(set! ,v ,e)
-     `(set-top-level! ,v ,(convert-assignments sfs e))]
-    ;bin op
-    [`(,o ,e1 ,e2)
-     #:when (op? o)
-     `(,o ,(convert-assignments sfs e1) ,(convert-assignments sfs e2))] 
+
+(define (ca prog)
+  (match prog
+    [`(store (,sfs ...) ,E [ ,e ])
+     (let ([as (get-assignments sfs E e)])
+       `(store ,(ca-sf-l sfs as) ,(ca-E E as) [ ,(ca-e e as) ]))]))
+
+(define (ca-sf-l sfs as)
+  (match sfs
+    ['() '()]
+    [`(,sf ,sfs1 ...) (cons (ca-sf sf as) (ca-sf-l sfs1 as))]))
+
+(define (ca-sf sf as)
+  (match sf
+    [`(,x ,v) `(,x (cons ,(ca-e v as) null))]
+    [u u]))
+
+(define (ca-E E as)
+  (match E
+    [`[] `[]]
+    [`(set! ,x ,E1) `(set-car! ,x ,(ca-E E1 as))]
+    [`(begin ,E1 ,e1 ,e2 ...) `(begin ,(ca-E E1 as) ,(ca-e e1 as) ,(ca-e-l e2 as))]
+    [`(,v1 ... ,E1 ,v2 ...) `(,(ca-e-l v1 as) ,(ca-E E1 as) ,(ca-e-l v2 as))]))
+
+(define (ca-e-l es as)
+  (match es
+    ['() '()]
+    [(cons e es1) (cons (ca-e e as)(ca-e-l es1 as))]))
+
+(define (ca-e e as)
+  (match e
+    [`(begin ,e1 ,e2 ...) `(begin ,(ca-e e1 as) ,(ca-e-l e2 as))]
+    [`(set! ,x ,e1) `(set-car! ,x ,(ca-e e1 as))]
     [x
-     x]))
+     #:when (member x as)
+     `(car ,x)]
+    [`(λ ,x ,e1)
+     #:when (member x as)
+     `(λ t ((λ ,x ,(ca-e e1 as))(cons t null)))]
+    [`(λ ,x ,e1)
+     #:when (not (member x as))
+     `(λ ,x ,(ca-e e1 as))]
+    [`(,e1 ,e2 ...) `(,(ca-e e1 as) ,(ca-e-l e2 as))]
+    [u u]))
 
+;x previously assigned
+(check-equal? (ca '(store ((x 4)) [] [ (begin null x) ]))
+              '(store ((x (cons 4 null))) [] [ (begin null ((car x))) ]))
 
-;canonical transformation example
-; '(let ([x v1])
-;   (set! x v2))
-; -->
-;'(let ([t v1])
-;   (let ([x (cons t '())])
-;     (set-car! x v2)))
+;x previously assigned and assigned again
+(check-equal? (ca '(store ((x 4)) [] [ (begin (set! x 5) x)]))
+              '(store ((x (cons 4 null))) [] [(begin (set-car! x 5) ((car x)))]))
 
-(check-equal? (convert-assignments '()
-                                   '(let v1
-                                      (bvar 0)))
-              '(let v1
-                 (bvar 0)))
+;y previously assigned, x not
+(check-equal? (ca '(store ((y 5)) [] [ (begin x y)]))
+              '(store ((y (cons 5 null))) [] [ (begin x ((car y)))]))
 
-(check-equal? (convert-assignments '()
-                                   '(let v1
-                                      (let v2
-                                        (bvar 0))))
-              '(let v1
-                 (let v2
-                   (bvar 0))))
+;x y both previously assigned
+(check-equal? (ca '(store ((x 3) (y 4)) [] [ (begin x y) ]))
+              '(store ((x (cons 3 null)) (y (cons 4 null))) [] [ (begin (car x) ((car y))) ]))
 
-(check-equal? (convert-assignments '()
-                                   '(let v1
-                                      (let v2
-                                        (bvar 0)
-                                        (bvar 1))))
-              '(let v1
-                 (let v2
-                   ((bvar 0)
-                   (bvar 1)))))
+;x assigned inside lambda
+(check-equal? (ca '(store () [] [ (λ x (set! x 4)) ]))
+              '(store () [] [ (λ t ((λ x (set-car! x 4))(cons t null))) ]))
 
+;x previously assigned, y assigned inside lambda in store
+(check-equal? (ca '(store ((x (λ y (set! y 5)))) [] [ x ]))
+              '(store ((x (cons (λ t ((λ y (set-car! y 5))(cons t null))) null))) [] [ (car x) ]))
 
-(check-equal? (convert-assignments '()
-                                   '(fvar x))
-              '(fvar x))
+;similar to above
+(check-equal? (ca '(store ((x (λ y (set! y 5)))) [] [ (begin x y) ]))
+              '(store ((x (cons (λ t ((λ y (set-car! y 5))(cons t null))) null))) [] [ (begin (car x) ((car y))) ]))
 
-(check-equal? (convert-assignments '()
-                                   '(let v1
-                                      (set! (bvar 0) v2)))
-              '(let v1
-                 (let (cons (bvar 0) '())
-                   (set-car! (bvar 0) v2))))
+;x assigned in eval context, also shows transforming eval context
+(check-equal? (ca '(store () ((λ x (set! x 4)) [] ) [ x ]))
+              '(store () (((λ t ((λ x (set-car! x 4))(cons t null)))) [] ()) [ (car x) ]))
 
-(check-equal? (convert-assignments '()
-                                    '(let v1
-                                       (set! (bvar 0) v2)
-                                       (bvar 0)))
-              '(let v1
-                 (let (cons (bvar 0) '())
-                   ((set-car! (bvar 0) v2)
-                   (car (bvar 0))))))
-
-(check-equal? (convert-assignments '()
-                                   '(let v1
-                                      (set! (bvar 1) v2)))
-              '(let v1
-                 (set-top-level! (bvar 1) v2)))
-
-(check-equal? (convert-assignments '()
-                                   '(let v1
-                                      (bvar 0)
-                                      (set! (bvar 0) v2)))
-              '(let v1
-                 (let (cons (bvar 0) '())
-                   ((car (bvar 0))
-                    (set-car! (bvar 0) v2)))))
-
-(define (ca-pass e)
-  (convert-assignments '() e))
-
-(define (no-sets? exp)
-  (match exp
-    [`(set! ,v ,e) #f]
-    [`(lam . ,body) (no-sets? body)]
-    [`(let ,v ,body) (no-sets? body)]
-    [`(let ,v ,body ...)
-     (and (map (lambda (e)
-                 (no-sets? e)) body))]
-    [`(,e1 ,e2)
-     (and (no-sets? e1) (no-sets? e2))] ;if app, handle both exprs
-    [_ #t]))
-                
+;x in store, transforms eval context
+(check-equal? (ca '(store ((x 4)) ((λ x x) [] ) [ x ]))
+              '(store ((x (cons 4 null))) (((λ t ((λ x (car x))(cons t null)))) [] () ) [ (car x) ]))
