Framework.v
@@ -1,4 +1,6 @@
 From vchez Require Import Definitions.
+From vchez Require Import Semantics.
+From vchez Require Import Helpers.
 From Coq Require Import List.
 From Metalib Require Import LibTactics.
 
@@ -58,9 +60,66 @@ Proof.
       + apply notin_union_2 in H. apply H.
       + apply notin_union_1 in H. apply H.
 Qed.
-    
-       
 
+(* programs are either values, stuck, or decompose uniquely into an ec and a reducible term *)
+Theorem unique_ec :
+  forall s t,
+  s_term t -> (* no standalone bvars *)
+  value t \/
+  ~(exists s' t', step s t s' t') \/
+  (exists C t' s' t'',
+    eval_ctx C ->
+    t = (C t') -> 
+    step s (C t') s' t'').
+Proof.
+  intros. 
+  induction t using s_trm_mutind. (* use our custom induction principle to get *)
+  - destruct x. (*s_trm_var case*)
+    + right. left. inversion H. (* standalone bvar -> False by s_term def *)
+    + right. right. (* standalone fvar steps to put itself in store *)  
+      exists (id). (* hole is just itself *)
+      exists (s_trm_var (fvar x)).
+      exists s.
+      exists (match (get_val x s) with
+              | SomeE v => v
+              | NoneE e => s_trm_err e
+              end).
+     intros. 
+     remember (get_val x s). destruct o.
+     * compute. apply step_var. symmetry. apply Heqo.
+     * compute. apply step_var_err. symmetry. apply Heqo.
+  - destruct IHt2. inversion H. apply H3.      
+       
+   try (left; repeat constructor).
+
+  
+  
+       
+Inductive vsr : sfs -> s_trm -> Prop :=
+  | vsr_val : forall s t, value t -> vsr s t
+  | vsr_stuck : forall s t, ~ (exists s' t', step s t s' t') -> vsr s t
+  | vsr_reducible : forall C s t,
+                    eval_ctx C ->
+                    (exists s' t', step s t s' t') -> 
+                    vsr s (C t).
+
+Theorem vsr_preserve :
+  forall s t,
+  vsr s t -> 
+  exists s' t', step s t s' t' ->
+  vsr s' t.
+Proof.
+  intros. induction t; simpl.
+Abort.
+
+
+  
+Theorem step_progress :
+  forall s t, s_term t -> value t \/ (exists s' t', step s t s' t').
+Proof.
+  intros. induction t; try (left; constructor); right.
+  - destruct ts.  
+  Abort.
      
     
     
